Fp/ExtraTheorems.lean
@@ -37,14 +37,12 @@ theorem toEFixed_isExactFloat (a : PackedFloat 5 2)
   bv_decide
 
 /--
-If a fixed point number is an exact floating point number, then converting to
+A fixed point number is an exact floating point number iff converting to
 floating point and back should not change the denotation.
 -/
-theorem isExactFloat_round_toEFixed (a : EFixedPoint 34 16) (m : RoundingMode)
-  (ha : isExactFloat 5 2 a)
-  : a.equal_denotation (round 5 2 m a).toEFixed := by
-  simp [isExactFloat, -BitVec.shiftLeft_eq', -BitVec.ushiftRight_eq'] at ha
-  simp [PackedFloat.toEFixed, round,
+theorem isExactFloat_iff_round_toEFixed (a : EFixedPoint 34 16) (m : RoundingMode)
+  : isExactFloat 5 2 a ↔ a.equal_denotation (round 5 2 m a).toEFixed := by
+  simp [isExactFloat, PackedFloat.toEFixed, round,
     -BitVec.shiftLeft_eq', -BitVec.ushiftRight_eq']
   bv_decide
 
@@ -112,11 +110,21 @@ operands are within a factor of two of each other.
 -/
 theorem sterbenz (a b : PackedFloat 5 2)
   (h : le a (doubleRNE b) ∧ le b (doubleRNE a))
-  : isExactFloat 5 2 (e_add .RTZ a.toEFixed ((neg b).toEFixed))
-  := by
+  : isExactFloat 5 2 (e_add .RTZ a.toEFixed ((neg b).toEFixed)) := by
   simp [le, doubleRNE] at h
   simp [e_add, f_add, neg, round, isExactFloat,
     PackedFloat.toEFixed,
+    -BitVec.shiftLeft_eq', -BitVec.ushiftRight_eq']
+  bv_decide
+
+-- Negation
+
+/--
+Negation will always map an exact float to an exact float.
+-/
+theorem neg_exact (a : PackedFloat 5 2)
+  : isExactFloat 5 2 (e_neg a.toEFixed) := by
+  simp [isExactFloat, e_neg, f_neg, PackedFloat.toEFixed,
     -BitVec.shiftLeft_eq', -BitVec.ushiftRight_eq']
   bv_decide
 
